feat(tmp/mini_crush): add experiments

tmp/mini_crush.lean
@@ -1,80 +1,57 @@
 declare_trace mini_crush
 
 namespace mini_crush
-open smt_tactic
+open smt_tactic tactic
 
-meta def snapshot := smt_state × tactic_state
+meta def is_auto_construction : name → bool
+| (name.mk_string "brec_on" p)      := tt
+| (name.mk_string "cases_on" p)     := tt
+| (name.mk_string "rec_on" p)       := tt
+| (name.mk_string "no_confusion" p) := tt
+| (name.mk_string "below" p)        := tt
+| _                                 := ff
 
-meta def save : smt_tactic snapshot :=
-smt_tactic.read
+meta def is_relevant_fn (n : name) : tactic bool :=
+do env ← get_env,
+   if ¬env^.is_definition n ∨ is_auto_construction n then return ff
+   else if env^.in_current_file n then return tt
+   else in_open_namespaces n
 
-meta def restore : snapshot → smt_tactic unit :=
-smt_tactic.write
-
-meta def try_and_save {α} (t : smt_tactic α) : smt_tactic (option (α × nat × snapshot)) :=
-do {
-  s     ← save,
-  a     ← t,
-  new_s ← save,
-  n     ← num_goals,
-  restore s,
-  return (a, n, new_s)
-} <|> return none
-
-meta def updt {α β} : option (α × nat × snapshot) → β → option (β × nat × snapshot)
-| none             b := none
-| (some (a, n, s)) b := some (b, n, s)
-
-meta def merge {α} (o₁ o₂ : option (α × nat × snapshot)) : option (α × nat × snapshot) :=
-match o₁, o₂ with
-| none,              _                 := o₂
-| _,                 none              := o₁
-| (some (_, n₁, _)), (some (_, n₂, _)) := if n₂ < n₁ then o₂ else o₁
-end
-
-meta def best_core {α} (ts : α → smt_tactic unit) : list α → option (α × nat × snapshot) → smt_tactic α
-| []      none             := failed
-| []      (some (v, _, s)) := restore s >> return v
-| (v::vs) b                := do
-  r ← try_and_save (ts v),
-  match r with
-  | some (_, 0, s) := restore s >> return v /- done -/
-  | _              := best_core vs (merge b (updt r v))
+meta def collect_revelant_fns_aux : name_set → expr → tactic name_set
+| s e :=
+e^.mfold s $ λ t _ s,
+  match t with
+  | expr.const c _ :=
+    if s^.contains c then return s
+    else mcond (is_relevant_fn c)
+      (do new_s ← return $ if c^.is_internal then s else s^.insert c,
+          d     ← get_decl c,
+          collect_revelant_fns_aux new_s d^.value)
+      (return s)
+  | _              := return s
   end
 
-meta def best {α} (vs : list α) (ts : α → smt_tactic unit) : smt_tactic α :=
-best_core ts vs none
+meta def collect_revelant_fns : tactic name_set :=
+do ctx ← local_context,
+   s₁  ← mfoldl (λ s e, infer_type e >>= collect_revelant_fns_aux s) mk_name_set ctx,
+   target >>= collect_revelant_fns_aux s₁
 
-open tactic (pp)
+meta def size (e : expr) : nat :=
+e^.fold 1 (λ e _ n, n+1)
 
-def nrounds := 5
+structure config :=
+(num_rounds := 5)
+(max_depth  := 2)
+(timeout    := 10000)
 
-meta def close_easy : smt_tactic unit :=
-all_goals (repeat_at_most nrounds (ematch >> try close))
+meta def close_easy (cfg : config) : smt_tactic unit :=
+all_goals (repeat_at_most cfg^.num_rounds (ematch >> try close))
 
-meta def destruct_and_close (e  : expr) : smt_tactic unit :=
-destruct e >> close_easy
+meta def destruct_and_close (cfg : config) (e : expr) : smt_tactic unit :=
+destruct e >> close_easy cfg
 
-meta def destruct_best (es : list expr) : smt_tactic expr :=
-do e ← best es $ λ e,
-          when_tracing `mini_crush (do p ← pp e, trace (to_fmt "[mini_crush] Candidate: " ++ p))
-       >> destruct_and_close e
-       >> when_tracing `mini_crush (do n ← num_goals, trace ("[mini_crush] Num goals: " ++ to_string n)),
-   when_tracing `mini_crush (do
-     p ← pp e,
-     tactic.trace (to_fmt "destructed: " ++ p)),
-   return e
-
-meta def induction_and_close (e : expr) : smt_tactic unit :=
-smt_tactic.induction e >> close_easy
-
-meta def induction_best (es : list expr) : smt_tactic expr :=
-best es induction_and_close
-
-meta def expr_set := expr_map unit
-meta def expr_set.mk := expr_map.mk unit
-meta def expr_set.insert (S : expr_set) (e : expr) : expr_set :=
-rb_map.insert S e ()
+meta def induction_and_close (cfg : config) (e : expr) : smt_tactic unit :=
+smt_tactic.induction e >> close_easy cfg
 
 open expr tactic
 
@@ -96,29 +73,371 @@ meta def collect_inductive_aux : expr_set → expr → tactic expr_set
     else return new_S
 
 meta def collect_inductive : expr → tactic expr_set :=
-collect_inductive_aux expr_set.mk
+collect_inductive_aux mk_expr_set
 
-meta def collect_inductive_as_list : tactic (list expr) :=
-do S ← target >>= collect_inductive, return $ S^.to_list^.for prod.fst
+meta def collect_inductive_from_target_aux : tactic (list expr) :=
+do S ← target >>= collect_inductive,
+   return $ list.qsort (λ e₁ e₂, size e₁ < size e₂) $ S^.to_list
+
+meta def collect_inductive_from_target : smt_tactic (list expr) :=
+collect_inductive_from_target_aux
+
+meta def snapshot := smt_state × tactic_state
+
+meta def save : smt_tactic snapshot :=
+smt_tactic.read
+
+meta def restore : snapshot → smt_tactic unit :=
+smt_tactic.write
+
+open smt_tactic
+
+meta def rsimp_target : smt_tactic unit :=
+do ccs ← to_cc_state,
+   rsimp.rsimplify_goal ccs
+
+meta def try_snapshots {α} (cont : α → smt_tactic unit) : list (α × snapshot) → smt_tactic unit
+| []           := failed
+| ((a, s)::ss) := (restore s >> cont a) <|> try_snapshots ss
+
+meta def search {α} (max_depth : nat) (act : nat → α → smt_tactic (list (α × snapshot))) : nat → α → smt_tactic unit
+| n s := do
+  all_goals $ try intros >> try close,
+  now
+  <|>
+  if n > max_depth then trace "max depth reached" >> trace_state >> failed
+  else all_goals $ try intros >> act n s >>= try_snapshots (search (n+1))
+
+meta def init_lemmas : smt_tactic unit :=
+do /- Add equational lemmas for relevant functions -/
+   fns ← collect_revelant_fns,
+   mfor' fns^.to_list add_ematch_eqn_lemmas_for,
+   /- Add [rsimp] lemmas -/
+   get_hinst_lemmas_for_attr `rsimp_attr >>= add_lemmas
+
+meta def try_induction_aux (hs : hinst_lemmas) (cont : smt_tactic unit) : list expr → smt_tactic unit
+| []      := failed
+| (e::es) := (induction e >> all_goals (set_lemmas hs >> try intros >> cont >> now)) <|> try_induction_aux es
+
+meta def try_induction (hs : hinst_lemmas) (cont : smt_tactic unit) : smt_tactic unit :=
+collect_inductive_from_target >>= mfilter (λ e, return $ e^.is_local_constant) >>= try_induction_aux hs cont
+
+meta def mini_crush_1 (cfg : config := {}) : tactic unit :=
+using_smt $ do
+  init_lemmas, hs ← get_lemmas,
+  close_easy cfg,
+  now
+  <|>
+  try_induction hs (close_easy cfg)
+
+universe variable u
+
+export nat (succ)
+
+def is_zero : ℕ → bool
+| 0        := tt
+| (succ _) := ff
+
+def plus : ℕ → ℕ → ℕ
+| 0 m         := m
+| (succ n') m := succ (plus n' m)
+
+def times : ℕ → ℕ → ℕ
+| 0        m := m
+| (succ n) m := plus m (times n m)
+
+@[simp] theorem n_plus_0 (n : ℕ) : plus n 0 = n :=
+by mini_crush_1
+
+@[simp] theorem plus_assoc (n1 n2 n3 : nat) : plus (plus n1 n2) n3 = plus n1 (plus n2 n3) :=
+by mini_crush_1
+
+inductive nat_list : Type
+| NNil  : nat_list
+| NCons : nat → nat_list → nat_list
+
+open nat_list
+
+def nlength : nat_list → ℕ
+| NNil          := 0
+| (NCons _ ls') := succ (nlength ls')
+
+def napp : nat_list → nat_list → nat_list
+| NNil ls2 := ls2
+| (NCons n ls1') ls2 := NCons n (napp ls1' ls2)
+
+theorem nlength_napp (ls1 ls2 : nat_list) : nlength (napp ls1 ls2) = plus (nlength ls1) (nlength ls2) :=
+by mini_crush_1
+
+inductive nat_btree : Type
+| NLeaf : nat_btree
+| NNode : nat_btree → ℕ → nat_btree → nat_btree
+
+open nat_btree
+
+def nsize : nat_btree → ℕ
+| NLeaf             := succ 0
+| (NNode tr1 _ tr2) := plus (nsize tr1) (nsize tr2)
+
+def nsplice : nat_btree → nat_btree → nat_btree
+| NLeaf tr2               := NNode tr2 0 NLeaf
+| (NNode tr1' n tr2') tr2 := NNode (nsplice tr1' tr2) n tr2'
+
+theorem nsize_nsplice (tr1 tr2 : nat_btree) : nsize (nsplice tr1 tr2) = plus (nsize tr2) (nsize tr1) :=
+by mini_crush_1
+
+inductive formula : Type
+| Eq     : nat → nat → formula
+| And    : formula → formula → formula
+| Forall : (nat → formula) → formula
+
+open formula
+
+example forall_refl : formula := Forall (λ x, Eq x x)
+
+def formula_denote : formula → Prop
+| (Eq n1 n2)  := n1 = n2
+| (And f1 f2) := formula_denote f1 ∧ formula_denote f2
+| (Forall f') := ∀ n : nat, formula_denote (f' n)
+
+def swapper : formula → formula
+| (Eq n1 n2)  := Eq n2 n1
+| (And f1 f2) := And (swapper f2) (swapper f1)
+| (Forall f') := Forall (λ n, swapper (f' n))
+
+attribute [simp] formula_denote swapper
+
+theorem swapper_preserves_truth (f) : formula_denote f → formula_denote (swapper f) :=
+by induction f; simph; intros; rsimp
+
+exit
+begin [smt] induction f, admit, admit, intros, init_lemmas, add_lemmas_from_facts, eblast, rsimp_target, intros, eblast, rsimp_target end
+
+exit
+
+begin [smt]
+  induction ls1,
+  init_lemmas, eblast
+
+end
+
+
+
+
+
+
+exit
+
+  (intros >> close >> now)
+  <|>
+  (if n > max_depth then (trace "max depth reached" >> rsimp >> trace_state)
+   else all_goals $ intros )
+
+
+exit
+    smt_tactic.intros >> collect_inductive_from_target >>= try_destruct cfg >>= try_snapshots (search (n+1))
+
+
+
+meta def try_and_save {α} (t : smt_tactic α) : smt_tactic (option (α × nat × snapshot)) :=
+do {
+  s     ← save,
+  a     ← t,
+  new_s ← save,
+  n     ← num_goals,
+  restore s,
+  return (a, n, new_s)
+} <|> return none
+
+meta def try_all_aux {α} (ts : α → smt_tactic unit) : list α → list (α × nat × snapshot) → smt_tactic (list (α × nat × snapshot))
+| []      [] := failed
+| []      rs := return rs^.reverse
+| (v::vs) rs := do
+  r ← try_and_save (ts v),
+  match r with
+  | some (_, 0, s) := return [(v, 0, s)]
+  | some (_, n, s) := try_all_aux vs ((v, n, s)::rs)
+  | none           := try_all_aux vs rs
+  end
+
+meta def try_all {α} (ts : α → smt_tactic unit) (vs : list α) : smt_tactic (list (α × nat × snapshot)) :=
+try_all_aux ts vs []
+
+meta def sort_snapshots (rs : list (expr × nat × snapshot)) : list snapshot :=
+let ss := flip list.qsort rs $ λ ⟨e₁, n₁, _⟩ ⟨e₂, n₂, _⟩, if n₁ ≠ n₂ then n₁ < n₂ else size e₁ < size e₂ in
+ss^.for $ λ ⟨_, _, s⟩, s
+
+meta def try_destruct (cfg : config) (es : list expr) : smt_tactic (list snapshot) :=
+sort_snapshots <$> try_all (destruct_and_close cfg) es
+
+meta def try_induction (cfg : config) (es : list expr) : smt_tactic (list snapshot) :=
+sort_snapshots <$> try_all (induction_and_close cfg) es
+
+meta def try_snapshots {α} (cont : smt_tactic α) : list snapshot → smt_tactic α
+| []      := failed
+| (s::ss) := (restore s >> cont) <|> try_snapshots ss
+
+meta def search (cfg : config) : nat → smt_tactic unit
+| n :=
+  close >> now
+  <|>
+  if n > cfg^.max_depth then trace "max depth reached" >> rsimp >> trace_state
+  else all_goals $
+    smt_tactic.intros >> collect_inductive_from_target >>= try_destruct cfg >>= try_snapshots (search (n+1))
+
+meta def with_smt (t : smt_tactic unit) : tactic unit :=
+using_smt_with {em_attr := `rsimp_attr} t
+
+meta def strategy_1 (cfg : config := {}) : tactic unit :=
+try_for cfg^.timeout (try simph >> try intros >> try simph >> try contradiction >> now)
+
+meta def strategy_2 (cfg : config := {}) : tactic unit :=
+try_for cfg^.timeout $ with_smt $
+  collect_inductive_from_target >>= try_induction cfg >>=
+  try_snapshots (all_goals $
+    trace "------------" >> trace_state >> now)
+
+-- exit
+--  try close >> try simph >> try intros >> try simph >>  try contradiction >> now)
+
+meta def strategy_3 (cfg : config := {}) : tactic unit :=
+try_for cfg^.timeout $ with_smt $
+  collect_inductive_from_target >>= try_induction cfg >>=
+  try_snapshots (all_goals $
+     trace "------------" >> trace_state >> trace "--------" >>
+     try close >> try (search cfg 1))
+
+meta def main (cfg : config := {}) : tactic unit :=
+strategy_2 <|> strategy_3
 
 end mini_crush
 
-/- Testing -/
-open smt_tactic mini_crush tactic
+meta def mini_crush := mini_crush.main
 
-lemma nil_append {α} (a : list α) : [] ++ a = a :=
-begin [smt]
-  collect_inductive_as_list >>= induction_best
-end
+universe variable u
 
-attribute [ematch_lhs] nil_append
+export nat (succ)
+
+def is_zero : ℕ → bool
+| 0        := tt
+| (succ _) := ff
+
+def plus : ℕ → ℕ → ℕ
+| 0 m         := m
+| (succ n') m := succ (plus n' m)
+
+def times : ℕ → ℕ → ℕ
+| 0        m := m
+| (succ n) m := plus m (times n m)
+
+attribute [simp] is_zero plus
 
 set_option trace.smt.ematch true
-set_option trace.mini_crush true
+
+theorem n_plus_0 (n : ℕ) : plus n 0 = n :=
+by mini_crush.strategy_3
+
+exit
+
+inductive nat_list : Type
+| NNil  : nat_list
+| NCons : nat → nat_list → nat_list
+
+open nat_list
+
+def nlength : nat_list → ℕ
+| NNil          := 0
+| (NCons _ ls') := succ (nlength ls')
+
+def napp : nat_list → nat_list → nat_list
+| NNil ls2 := ls2
+| (NCons n ls1') ls2 := NCons n (napp ls1' ls2)
+
+attribute [simp] nlength napp
+
+theorem nlength_napp (ls1 ls2 : nat_list) : nlength (napp ls1 ls2) = plus (nlength ls1) (nlength ls2) :=
+by induction ls1; rsimp
+
+inductive nat_btree : Type
+| NLeaf : nat_btree
+| NNode : nat_btree → ℕ → nat_btree → nat_btree
+
+open nat_btree
+
+def nsize : nat_btree → ℕ
+| NLeaf             := succ 0
+| (NNode tr1 _ tr2) := plus (nsize tr1) (nsize tr2)
+
+def nsplice : nat_btree → nat_btree → nat_btree
+| NLeaf tr2               := NNode tr2 0 NLeaf
+| (NNode tr1' n tr2') tr2 := NNode (nsplice tr1' tr2) n tr2'
+
+attribute [simp] nsize nsplice
+
+theorem plus_assoc (n1 n2 n3 : nat) : plus (plus n1 n2) n3 = plus n1 (plus n2 n3) :=
+by induction n1; simph
+
+attribute [simp] n_plus_0 plus_assoc
+
+theorem nsize_nsplice (tr1 tr2 : nat_btree) : nsize (nsplice tr1 tr2) = plus (nsize tr2) (nsize tr1) :=
+by induction tr1; simph
+
+export list (nil cons)
+
+def length {α : Type u} : list α → ℕ
+| nil          := 0
+| (cons _ ls') := succ (length ls')
+
+def app {α : Type u} : list α → list α → list α
+| nil ls2           := ls2
+| (cons x ls1') ls2 := cons x (app ls1' ls2)
+
+attribute [simp] length app
+
+theorem length_app {α : Type u} (ls1 ls2 : list α) : length (app ls1 ls2) = plus (length ls1) (length ls2) :=
+by induction ls1; simph
 
 
-example (a b c : list nat) : (a ++ []) ++ b = a ++ b :=
-begin [smt]
-  do { monad.mapm to_expr [`(b), `(a), `(c)] >>= destruct_best },
+inductive pformula : Type
+| Truth : pformula
+| Falsehood : pformula
+| Conjunction : pformula → pformula → pformula.
+
+open pformula
+
+def pformula_denote : pformula → Prop
+| Truth               := true
+| Falsehood           := false
+| (Conjunction f1 f2) := pformula_denote f1 ∧ pformula_denote f2
+
+attribute [simp] pformula_denote
+
+open pformula
+
+inductive formula : Type
+| Eq     : nat → nat → formula
+| And    : formula → formula → formula
+| Forall : (nat → formula) → formula
+
+open formula
+
+example forall_refl : formula := Forall (λ x, Eq x x)
+
+def formula_denote : formula → Prop
+| (Eq n1 n2)  := n1 = n2
+| (And f1 f2) := formula_denote f1 ∧ formula_denote f2
+| (Forall f') := ∀ n : nat, formula_denote (f' n)
+
+def swapper : formula → formula
+| (Eq n1 n2)  := Eq n2 n1
+| (And f1 f2) := And (swapper f2) (swapper f1)
+| (Forall f') := Forall (λ n, swapper (f' n))
+
+attribute [simp] formula_denote swapper
+
+theorem swapper_preserves_truth (f) : formula_denote f → formula_denote (swapper f) :=
+begin
+  (do s ← mini_crush.collect_revelant_fns, tactic.trace s^.to_list),
+  induction f; intro h; simp at h; simph; intros; rsimp
 
 end
